Source/DafnyCore/Resolver/PreType/PreTypeResolve.Statements.cs
@@ -1134,7 +1134,7 @@ namespace Microsoft.Dafny {
           //     nat^N -> rr.EType  :>  rr.ElementInit.Type
           resolver.SystemModuleManager.CreateArrowTypeDecl(dims);  // TODO: should this be done already in the parser?
           var indexPreTypes = Enumerable.Repeat(Type2PreType(resolver.SystemModuleManager.Nat()), dims).ToList();
-          var arrowPreType = BuiltInArrowType(indexPreTypes, elementPreType);
+          var arrowPreType = BuiltInArrowType(indexPreTypes, elementPreType, true, true);
           Constraints.AddSubtypeConstraint(arrowPreType, rr.ElementInit.PreType, rr.ElementInit.Origin, () => {
             var hintString = !PreType.Same(arrowPreType, rr.ElementInit.PreType) ? "" :
               string.Format(" (perhaps write '{0} =>' in front of the expression you gave in order to make it an arrow type)",
